A in A->B is (A'->B'), i.e., retention of A'->B'.

And A' in A'->B' is (A''->B''), i.e., retenton of A''->B''.

And the same applies hereafter.

Now we consider the form of the semiosis ((((...)->B''')->B'')->B')->B by identifying all of B, B', B'', B''',... as b.

We then define a function s(x) of x as s(x) ≡ (x)->b.

We refer the fixed point of s(x) as a.

a satisfies s(a) = a. 

Therefore, it holds that a = (a)->b. And it also holds that a = ((a)->b)->b. And the same applies hereafter.

The fixed point of s(x) is the very form of the nesting structure of semiosis.

The function s(x) is being given direction (donné sens) by retention of x to some coming signifier.
